theories/models/utp_vdm_simple/examples/Dwarf.thy
@@ -86,6 +86,21 @@ definition "extinguish = MkChanD ''extinguish'' \<parallel>@LampId\<parallel>"
 definition "setPS = MkChanD ''setPS'' \<parallel>@ProperState\<parallel>"
 definition "shine = MkChanD ''shine'' \<parallel>@Signal\<parallel>"
 
+(* FIXME: Execution of CML operations needs to take care of undefinedness *)
+
+lift_definition Exec1D :: 
+  "('a \<Rightarrow> vdmv WF_PREDICATE) \<Rightarrow> 'a vdme \<Rightarrow> vdmv WF_PREDICATE" 
+  is "\<lambda> P e. {b :: vdmv WF_BINDING. b \<in> P (the (e b))}" .
+
+syntax
+  "_cml_exec1" :: "idt \<Rightarrow> pexpr \<Rightarrow> upred" ("_'(_')")
+
+translations
+  "_cml_exec1 f s" == "CONST Exec1D f s"
+
+locale DwarfProcess
+begin
+
 definition "dw \<equiv> MkVarD ''dw'' DwarfType"
 
 definition "DwarfInv \<equiv> `\<lparr> $dw hasType @DwarfType \<rparr> \<turnstile> \<lparr> $dw\<acute> hasType @DwarfType \<rparr>`"
@@ -130,34 +145,13 @@ definition
                           , ($dw).currentstate setminus {^l^}
                           , ($dw).desiredproperstate)`"
 
-(* FIXME: Execution of CML operations needs to take care of undefinedness *)
-
-lift_definition Exec1D :: 
-  "('a \<Rightarrow> vdmv WF_PREDICATE) \<Rightarrow> 'a vdme \<Rightarrow> vdmv WF_PREDICATE" 
-  is "\<lambda> P e. {b :: vdmv WF_BINDING. b \<in> P (the (e b))}" .
-
-syntax
-  "_dwarf_turnon" :: "pexpr \<Rightarrow> upred" ("TurnOn'(_')")
-
-translations
-  "_dwarf_turnon l" == "CONST Exec1D CONST TurnOn l"
-
-term "`(light?(l) \<rightarrow> TurnOn(&l)) ; DWARF`"
 
 definition 
-  "DWARF =
-    (  (light?l -> TurnOn(l); DWARF) 
-    [] (extinguish?l -> TurnOff(l); DWARF)
-    [] (setPS?l -> SetNewProperState(l); DWARF)
-    [] (shine!(dw.currentstate) -> DWARF))"
-
-
-term "EventPE init UnitD"
-
-term "|setPS.({<L1>,<L2>})|"
-
-
-term "`setPS.({}) \<rightarrow> SKIP`"
+  "DWAFT = `\<mu> DWARF. 
+          (((light?(l) -> TurnOn(&l)) ; DWARF) 
+       [] ((extinguish?(l) -> TurnOff(&l)); DWARF)
+       [] ((setPS?(s) -> SetNewProperState(&s)); DWARF)
+       [] (shine!(($dw).currentstate) -> DWARF))`"
 
 end
 
